update show files for some defs.v tests

tree-automata/defs_tests/lemma_prec_c_int1_302/show_prec_list.v
@@ -1,16 +1,25 @@
-From QuickChick Require Import QuickChick Tactics.
-Import QcNotation.
-Require Import Ndec.
-
-Require Import Bool.
-Require Import Arith.
-Require Import ZArith.
-Require Import NArith.
-Require Import EqNat.
-Require Import Ndigits.
-Require Import Ndec.
-
 Open Scope string_scope.
+
+Definition show_type_name_BV (T : Type) := 
+  match T with
+  | bool => "bool"
+  end.
+
+Instance show_BV {T} `{_ : Show T} : Show (list T) := 
+{| show := 
+     let fix aux l :=
+       match l with
+       | nil => "@nil (" ++ show_type_name_BV T ++ ")" 
+       | cons x xs => "@cons (" ++ show_type_name_BV T ++ ") " ++ show x ++ " (" ++ aux xs ++ ")"
+       end
+      in aux
+|}.
+Derive Arbitrary for list.
+Instance Dec_Eq_BV {T} `{_ : Dec_Eq T}  : Dec_Eq (list T).
+Proof. dec_eq. Qed.
+
+(* Start tree-automata stuff *)
+
 Fixpoint show_pos p :=
     match p with
     | xH => "xH"
@@ -24,13 +33,205 @@ Definition show_N n :=
     | Npos p => "Npos (" ++ show_pos p ++ ")"
     end.
 
-Definition ad := N. 
-Notation Neqb := N.eqb.
 Instance show_ad : Show ad := {| show := show_N |}.
 
-Inductive prec_list : Set :=
-  | prec_cons : ad -> prec_list -> prec_list -> prec_list
-  | prec_empty : prec_list.
+
+(* Map Instances *)
+Instance show_map {A} `{_ : Show A} : Show (Map A) :=
+{| show := 
+    let fix aux l := 
+        match l with
+        | M0 => "M0"
+        | M1 a b => "M1 (" ++ show a ++ ")(" ++ show b ++ ")"
+        | M2 x y => "M2 (" ++ aux x ++ ") (" ++ aux y ++ ")"
+        end
+    in aux 
+|}.
+
+Derive Arbitrary for positive.
+Derive Arbitrary for N.
+
+Definition genM0 {A} := M0 A.
+Definition genM1 {A} := M1 A.
+Definition genM2 {A} := M2 A.
+
+(* (Map A) in typeclass GenSized *)
+Definition genMap {A} (g : G A) : nat -> G (Map A) := 
+    let fix aux sz := 
+        match sz with
+        | O => ret genM0
+        | S z => 
+            freq [
+                (0, ret genM0) ; 
+                (1, liftM2 genM1 arbitrary g) ; 
+                (sz, liftM2 genM2 (aux z) (aux z))
+            ]
+        end
+    in aux.
+
+
+Definition genMapBounded {A} (g : G A) : G (Map A) := sized (genMap g).
+Definition mapShrink {A} (x : A) := (@nil A).
+
+Instance genMapInstanceGen {A} `{_ : Gen A} : Gen (Map A) := {| arbitrary := genMapBounded arbitrary |}.
+Instance genMapInstanceShrink {A} : Shrink (Map A) := {| shrink := mapShrink |}.
+
+Set Nested Proofs Allowed.
+Instance Dec_Eq_map {A} `{_ : Dec_Eq A} : Dec_Eq (Map A).
+Proof. dec_eq. Qed.
+
+(* Terms and Term_List Instances *)
+Fixpoint show_term_fix t := 
+    match t with
+    | app a tl => "app (" ++ show a ++ ") (" ++ show_term_list_fix tl ++ ")"
+    end 
+with show_term_list_fix tl :=
+    match tl with
+    | tnil => "tnil"
+    | tcons t l =>"tcons (" ++ show_term_fix t ++ ") (" ++ show_term_list_fix l ++ ")"
+    end.
+
+Instance show_term : Show (term) := {| show := show_term_fix |}.
+Instance show_term_list : Show (term_list) := {| show := show_term_list_fix |}.
+
+Fixpoint genTerm sz : G (term) := 
+    match sz with
+    | O => liftM2 app arbitrary (ret tnil)
+    | S z => 
+        freq [
+            (0, liftM2 app arbitrary (ret tnil)) ; 
+            (sz, liftM2 app arbitrary (genTermList z))
+        ]
+    end
+with genTermList zs : G (term_list) :=
+    match zs with
+    | O => ret tnil
+    | S z => 
+        freq [
+            (0, ret tnil) ; 
+            (1, liftM2 tcons (genTerm z) (ret tnil)) ; 
+            (zs, liftM2 tcons (genTerm z) (genTermList z))
+        ]
+    end.
+
+(* (Map A) in typeclass Gen *)
+Definition genTermSized : G (term) := sized (genTerm).
+Definition genTermListSized : G (term_list) := sized (genTermList).
+
+(* (Map A) in the Shrink typeclass*)
+Definition shrinkGen {A} (x : A) := (@nil A).
+
+Instance genTermListInstanceGen : Gen (term_list) := {| arbitrary := genTermListSized |}.
+Instance genTermListInstanceShrink : Shrink (term_list) := {| shrink := shrinkGen |}.
+
+Instance genTermInstanceGen : Gen (term) := {| arbitrary := genTermSized |}.
+Instance genTermInstanceShrink : Shrink (term) := {| shrink := shrinkGen |}.
+
+Definition term_list_ind2 (P : term_list -> Prop) (f : P tnil)
+  (f0 : (forall (a : ad) (l : term_list) (l0 : term_list), P l -> P l0 -> P (tcons (app a l) l0))) :=
+fix F (t : term_list) : P t :=
+  match t as t0 return (P t0) with
+  | tnil => f
+  | tcons (app a0 t0) t1 => f0 a0 t0 t1 (F t0) (F t1)
+  end.
+
+(* This is unchanged from what you had. *)
+Fixpoint term_eqb (t1 t2 : term) : bool :=
+    match t1,t2 with
+    | app a1 l1, app a2 l2  => andb (Neqb a1 a2) (term_list_eqb l1 l2)
+    end
+with term_list_eqb (l1 l2 : term_list) : bool :=
+    match l1,l2 with
+    | tnil, tnil => true
+    | tcons t1 n1, tcons t2 n2 => andb (term_eqb t1 t2) (term_list_eqb n1 n2)
+    | _, _ => false
+    end.
+
+Lemma if_term_list_eqb : forall l1 l2, term_list_eqb l1 l2 = true -> l1 = l2.
+Proof.
+intro l1.
+induction l1 using term_list_ind2. destruct l2. 
+    auto.
+    simpl. intros. contradict H. auto.
+destruct l2.
+    simpl. intros. contradict H. auto.
+    intro. destruct t. simpl in H.
+    assert ((Neqb a a0 = true) /\ (term_list_eqb l1_1 t = true) /\ (term_list_eqb l1_2 l2) = true).
+    destruct (Neqb a a0). destruct (term_list_eqb l1_1 t). destruct (term_list_eqb l1_2 l2).
+    - split. reflexivity. split. reflexivity. reflexivity.
+    - simpl in H. contradict H. auto.
+    - simpl in H. contradict H. auto.
+    - simpl in H. contradict H. auto.
+    - inversion H0. inversion H2.
+    assert (a = a0). apply Neqb_complete. assumption. rewrite H5.
+    assert (l1_1 = t). apply IHl1_1. assumption. rewrite H6.
+    assert (l1_2 = l2). apply IHl1_2. assumption. rewrite H7.
+    reflexivity.
+Qed.
+
+Lemma eq_tcons_def (t1 t2 : term) (l1 l2 : term_list) : ((t1 = t2) /\ (l1 = l2)) <-> ((tcons t1 l1) = (tcons t2 l2)).
+Proof.
+    intros. split.
+    - intros. destruct H. rewrite H. rewrite H0. auto.
+    - intros. inversion H. auto.
+Qed.
+
+Lemma term_list_eqb_refl : forall l, term_list_eqb l l = true.
+Proof.
+    intros. induction l using term_list_ind2.
+    - auto.
+    - simpl term_list_eqb.
+    assert (G1: Neqb a a = true). apply Neqb_correct.
+    rewrite G1. rewrite IHl1. rewrite IHl2. auto.
+Qed.
+
+Lemma fi_term_list_eqb : forall l1 l2, l1 = l2 -> term_list_eqb l1 l2 = true.
+Proof.
+    intros. rewrite H. induction l2 using term_list_ind2.
+    - auto.
+    - simpl.
+    assert (G1: Neqb a a = true). apply Neqb_correct.
+    rewrite G1. simpl. rewrite term_list_eqb_refl. rewrite term_list_eqb_refl. auto.
+Qed.
+
+Theorem term_list_Eq_eq : forall l1 l2, term_list_eqb l1 l2 = true <-> l1 = l2.
+Proof. split. apply if_term_list_eqb. apply fi_term_list_eqb. Qed.
+
+Lemma eq_terms_def (a1 a2 : ad) (t1 t2 : term_list) : ((a1 = a2) /\ (t1 = t2)) <-> ((app a1 t1) = (app a2 t2)).
+Proof. 
+    intros. split.
+    - intros. destruct H. rewrite H. rewrite H0. auto.
+    - intros. inversion H. auto. 
+Qed.
+
+Theorem term_Eq_eq (t1 t2 : term) : term_eqb t1 t2 = true <-> t1 = t2.
+Proof.
+    split.
+    * intros. destruct t1; destruct t2. rewrite <- eq_terms_def. inversion H. apply andb_prop in H1.
+    destruct H1. apply Neqb_complete in H0. rewrite term_list_Eq_eq in H1. auto.
+    * intros. destruct t1; destruct t2. simpl. inversion H.  
+    assert (G1: Neqb a0 a0 = true). apply Neqb_correct.
+    rewrite G1. simpl. rewrite term_list_eqb_refl. auto.
+Qed. 
+
+Lemma add_neqb (b : bool) : b = false -> ~b = true.
+Proof. destruct b. intros. inversion H. intros. auto. Qed.
+
+Instance Dec_Eq_term : Dec_Eq term.
+Proof.
+ constructor. intros. unfold ssrbool.decidable. destruct (term_eqb x y) eqn:H.
+ - left. apply term_Eq_eq. apply H.
+ - right. apply add_neqb in H. unfold not. rewrite <- term_Eq_eq. intros. contradiction.   
+ Qed.
+
+Instance Dec_Eq_term_list : Dec_Eq term_list.
+ Proof.
+  constructor. intros. unfold ssrbool.decidable. destruct (term_list_eqb x y) eqn:H.
+  - left. apply term_list_Eq_eq. apply H.
+  - right. apply add_neqb in H. unfold not. rewrite <- term_list_Eq_eq. intros. contradiction.
+ Qed.
+
+(* Prec_list Instances *)
 
 Fixpoint show_prec_list_fix p := 
     match p with
@@ -108,4 +309,233 @@ Proof.
     destruct (prec_list_eqb x y) eqn:E.
     - apply if_prec_cons_eq in E. auto.
     - right. apply add_neqb in E.  unfold not. intros. apply fi_prec_cons_eq in H. contradiction.
+Qed.
+
+(* State and DTA Instances *)
+
+Instance Dec_Eq_state : Dec_Eq state. Proof. dec_eq. Qed.
+Instance Dec_Eq_preDTA : Dec_Eq preDTA. Proof. dec_eq. Qed.
+Instance Dec_Eq_DTA : Dec_Eq DTA. Proof. dec_eq. Qed.
+
+Definition genState : nat -> G (state) := genMap arbitrary.
+Definition genStateBounded : G (state) := sized (genState).
+Instance genStateInstanceGen : Gen (state) := {| arbitrary := genStateBounded |}.
+Instance genStateInstanceShrink : Shrink (state) := {| shrink := mapShrink |}.
+
+Definition genPreDTA : nat -> G (preDTA) := genMap arbitrary.
+Definition genPreDTABounded : G (preDTA) := sized (genPreDTA).
+Instance genPreDTAInstanceGen : Gen (preDTA) := {| arbitrary := genPreDTABounded |}.
+Instance genPreDTAInstanceShrink : Shrink (preDTA) := {| shrink := mapShrink |}.
+
+Definition genDTABounded : G (DTA) := liftM2 dta genPreDTABounded arbitrary.
+Instance genDTAInstanceGen : Gen (DTA) := {| arbitrary := genDTABounded |}.
+Instance genDTAInstanceShrink : Shrink (DTA) := {| shrink := mapShrink |}.
+
+Fixpoint show_state_fix s := 
+    match s with
+    | M0 => "M0 prec_list"
+    | M1 a p => "M1 prec_list (" ++ show_N a ++ ") (" ++ show_prec_list_fix p ++ ")"
+    | M2 s1 s2 => "M2 prec_list (" ++ show_state_fix s1 ++ ") (" ++ show_state_fix s2 ++ ")"
+    end.
+
+Fixpoint show_PreDTA_fix s := 
+    match s with
+    | M0 => "M0 state"
+    | M1 a p => "M1 state (" ++ show_N a ++ ") (" ++ show_state_fix p ++ ")"
+    | M2 s1 s2 => "M2 state (" ++ show_PreDTA_fix s1 ++ ") (" ++ show_PreDTA_fix s2 ++ ")"
+    end.
+
+Fixpoint show_DTA_fix d := 
+    match d with dta p a => "dta (" ++ show_PreDTA_fix p ++ ") (" ++ show_N a ++ ")" end.
+
+Instance show_state : Show (state) := {| show := show_state_fix |}.
+Instance show_predta : Show (preDTA) := {| show := show_PreDTA_fix |}.
+Instance show_dta : Show (DTA) := {| show := show_DTA_fix |}.
+
+Instance Dec_prec_occur (a : ad) (p : prec_list) : Dec (prec_occur p a).
+Proof. 
+    dec_eq.
+    induction p.
+    - destruct (Neqb a a0) eqn:E.
+    + apply Neqb_complete in E. rewrite E. left. apply prec_hd.
+    + destruct IHp1.
+    * left. apply prec_int0. auto.
+    * destruct IHp2.
+    ** left. apply prec_int1. auto.
+    ** right. unfold not; intros. inversion H.
+    *** rewrite H0 in E. rewrite Neqb_correct in E. discriminate E.
+    *** unfold not in n. apply n. auto.
+    *** unfold not in n0. apply n0. auto.
+    - right. unfold not. intros. inversion H.
+Qed.
+
+Instance Dec_prec_contained (p q : prec_list) : Dec (prec_contained p q).
+Proof.
+    dec_eq.
+    induction q.
+    - destruct (prec_list_eqb p (prec_cons a q1 q2)) eqn:E.
+    + left. apply if_prec_cons_eq in E. rewrite E. apply prec_id.
+    + inversion IHq1.
+    * left. apply prec_c_int0. auto.
+    * inversion IHq2.
+    ** left. apply prec_c_int1. auto.
+    ** right. unfold not; intros. inversion H1.
+    *** rewrite H3 in E. rewrite prec_list_eqb_refl in E. discriminate E.
+    *** unfold not in H. apply H. auto.
+    *** unfold not in H0. apply H0. auto.
+    - induction p.
+    -- right. unfold not; intros. inversion H.
+    -- left. apply prec_id.
+Qed.
+
+Instance Dec_prec_in_state (s : state) (p : prec_list) : Dec (prec_in_state s p).
+Proof. 
+    dec_eq. unfold prec_in_state. induction s.
+    - right. unfold not. intros. inversion H. discriminate H0.
+    - destruct (prec_list_eqb a0 p) eqn:E.
+    + apply if_prec_cons_eq in E. rewrite E. left. exists a. simpl. rewrite Neqb_correct. auto.
+    + right. unfold not. intros. inversion H. destruct (Neqb a x) eqn:F.
+    * apply Neqb_complete in F. rewrite F in H0. simpl in H0. rewrite Neqb_correct in H0.
+    inversion H0. apply fi_prec_cons_eq in H2. rewrite H2 in E. discriminate E.
+    * simpl in H0. rewrite F in H0. discriminate H0.
+    - inversion IHs1.
+    + left. inversion H. exists (N.double x). 
+    assert (A: exists b, b = Ndouble x). exists (N.double x). auto. inversion A.
+    assert (B: x0 = Ndouble x -> N.div2 x0 = x). intros. rewrite H1. simpl. apply N.div2_double.
+    assert (C: Ndiv2 x0 = x). apply B. apply H1. 
+    rewrite <- H0. rewrite <- H1. rewrite <- C. apply MapGet_M2_bit_0_0.
+    rewrite H1. apply Ndouble_bit0.
+    + inversion IHs2.
+    ++ left. inversion H0. exists (N.succ_double x).
+    assert (A: exists b, b = N.succ_double x). exists (N.succ_double x). auto. inversion A.
+    assert (B: x0 = N.succ_double x -> N.div2 x0 = x). intros. rewrite H2. apply N.div2_succ_double.
+    assert (C: Ndiv2 x0 = x). apply B. apply H2. inversion A.
+    rewrite <- H1. rewrite <- H2. rewrite <- C. apply MapGet_M2_bit_0_1. rewrite H2. apply Ndouble_plus_one_bit0.
+    ++ right. unfold not. intros. inversion H1. destruct (N.odd x) eqn:E.
+    +++ unfold not in H0. apply H0. exists (N.div2 x). rewrite <- H2. apply eq_sym. apply MapGet_M2_bit_0_1. auto.
+    +++ unfold not in H. apply H. exists (N.div2 x). rewrite <- H2. apply eq_sym. apply MapGet_M2_bit_0_0. auto.
+Qed.
+
+Fixpoint taille_0 (l : prec_list) : nat :=
+  match l with
+  | prec_empty => 0
+  | prec_cons x y z => S (taille_0 y + taille_0 z)
+  end.
+
+Fixpoint taille_1 (s : state) : nat :=
+  match s with
+  | M0 => 0
+  | M1 x y => taille_0 y
+  | M2 x y => max (taille_1 x) (taille_1 y)
+  end.
+
+Definition smaller (s s1 s2 : state) : bool := (andb (Nat.leb (taille_1 s1) (taille_1 s)) (Nat.leb (taille_1 s2) (taille_1 s))).
+
+Fixpoint state_eqb (s1 s2 : state) : bool :=
+    match s1,s2 with
+    | M0, M0 => true
+    | M1 a1 p1, M1 a2 p2 => andb (Neqb a1 a2) (prec_list_eqb p1 p2)
+    | M2 s1_1 s1_2, M2 s2_1 s2_2 => 
+        andb (andb (smaller s1 s1_1 s1_2)  (smaller s2 s2_1 s2_2))  (andb (state_eqb s1_1 s2_1) (state_eqb s1_2 s2_2))
+    |_,_ => false
+    end.
+
+Lemma if_state_eq : forall s1 s2, state_eqb s1 s2 = true -> s1 = s2.
+Proof.
+    induction s1.
+    - destruct s2. 
+    -- auto.
+    -- simpl. intros. inversion H.
+    -- simpl. intros. inversion H.
+    - destruct s2.
+    -- simpl. intros. inversion H.
+    -- simpl. intros. apply andb_true_iff in H. destruct H. apply Neqb_complete in H.
+    apply if_prec_cons_eq in H0. rewrite H; rewrite H0. reflexivity.
+    -- simpl. intros. inversion H.
+    - destruct s2. 
+    -- simpl. intros. inversion H.
+    -- simpl. intros. inversion H.
+    -- intros. inversion H. apply andb_true_iff in H1. destruct H1.
+    apply andb_true_iff in H1. destruct H1. apply andb_true_iff in H0. destruct H0.
+    apply IHs1_1 in H1. apply IHs1_2 in H2. rewrite H1. rewrite H2. reflexivity.
+Qed.
+
+Lemma leb_max_l : forall n m, n <=? max n m = true.
+Proof.
+    intros. apply Nat.leb_le. generalize dependent n. induction m.
+    - destruct n. auto. auto.
+    - simpl. destruct n. apply le_0_n. simpl. transitivity (S (max n m)). 
+    apply le_n_S. apply IHm. auto.
+Qed.  
+
+Lemma leb_max_r : forall n m, m <=? max n m = true.
+Proof.
+    intros. apply Nat.leb_le. generalize dependent m. induction n.
+    - destruct m. auto. auto.
+    - simpl. destruct m. apply le_0_n. simpl. transitivity (S (max n m)). 
+    apply le_n_S. apply IHn. auto.
 Qed. 
+
+Lemma smaller_self: forall s1 s2, smaller (M2 prec_list s1 s2) s1 s2 = true.
+Proof.
+    intros. unfold smaller. simpl. apply andb_true_iff. split.
+    apply leb_max_l. apply leb_max_r.
+Qed.
+
+Lemma state_eqb_refl : forall s, state_eqb s s = true.
+Proof.
+    induction s. 
+    - auto. 
+    - simpl. apply andb_true_iff. split. apply Neqb_correct. apply prec_list_eqb_refl.
+    - simpl. apply andb_true_iff. split. 
+    -- apply andb_true_iff. split. apply smaller_self. apply smaller_self.
+    -- apply andb_true_iff. split. auto. auto.
+Qed.   
+
+Lemma fi_state_eq : forall s1 s2, s1 = s2 -> state_eqb s1 s2 = true.
+Proof. intros. rewrite H. apply state_eqb_refl. Qed. 
+
+Lemma state_eq_iff : forall s1 s2, s1 = s2 <-> state_eqb s1 s2 = true.
+Proof. split. apply fi_state_eq. apply if_state_eq. Qed.
+
+Instance Dec_state_in_dta (s : state) (d : preDTA) : Dec (state_in_dta d s).
+Proof. 
+    dec_eq. unfold state_in_dta. induction d.
+    - right. unfold not. intros. inversion H. discriminate H0.
+    - destruct (state_eqb a0 s) eqn:E.
+    + apply state_eq_iff in E. rewrite E. left. exists a. simpl. rewrite Neqb_correct. auto.
+    + right. unfold not. intros. inversion H. destruct (Neqb a x) eqn:F.
+    * apply Neqb_complete in F. rewrite F in H0. simpl in H0. rewrite Neqb_correct in H0.
+    inversion H0. apply state_eq_iff in H2. rewrite H2 in E. discriminate E.
+    * simpl in H0. rewrite F in H0. discriminate H0.
+    - inversion IHd1.
+    + left. inversion H. exists (N.double x). 
+    assert (A: exists b, b = Ndouble x). exists (N.double x). auto. inversion A.
+    assert (B: x0 = Ndouble x -> N.div2 x0 = x). intros. rewrite H1. simpl. apply N.div2_double.
+    assert (C: Ndiv2 x0 = x). apply B. apply H1. 
+    rewrite <- H0. rewrite <- H1. rewrite <- C. apply MapGet_M2_bit_0_0.
+    rewrite H1. apply Ndouble_bit0.
+    + inversion IHd2.
+    ++ left. inversion H0. exists (N.succ_double x).
+    assert (A: exists b, b = N.succ_double x). exists (N.succ_double x). auto. inversion A.
+    assert (B: x0 = N.succ_double x -> N.div2 x0 = x). intros. rewrite H2. apply N.div2_succ_double.
+    assert (C: Ndiv2 x0 = x). apply B. apply H2. inversion A.
+    rewrite <- H1. rewrite <- H2. rewrite <- C. apply MapGet_M2_bit_0_1. rewrite H2. apply Ndouble_plus_one_bit0.
+    ++ right. unfold not. intros. inversion H1. destruct (N.odd x) eqn:E.
+    +++ unfold not in H0. apply H0. exists (N.div2 x). rewrite <- H2. apply eq_sym. apply MapGet_M2_bit_0_1. auto.
+    +++ unfold not in H. apply H. exists (N.div2 x). rewrite <- H2. apply eq_sym. apply MapGet_M2_bit_0_0. auto.
+Qed.
+
+(* Option instance *)
+Instance show_option {A} `{_ : Show A} : Show (option A) :=
+{| show := 
+    let fix aux l := 
+        match l with
+        | None => "None"
+        | Some x => "Some ("++ show x ++")"
+        end
+    in aux 
+|}.
+Derive Arbitrary for option.
+Instance Dec_Eq_option {A} `{_ : Dec_Eq A} : Dec_Eq (option A).
+Proof. dec_eq. Qed.
